BV/BVConform.thy
@@ -33,11 +33,6 @@ abbreviation
 notation (ASCII)
   confTs  ("_,_ |- _ [:<=T] _" [51,51,51,51] 50)
 
-(* HERE: MOVE*)
-abbreviation Called_set :: "instr set" where
-"Called_set \<equiv> {i. \<exists>C. i = New C} \<union> {i. \<exists>C M n. i = Invokestatic C M n}
-                 \<union> {i. \<exists>C F D. i = Getstatic C F D} \<union> {i. \<exists>C F D. i = Putstatic C F D}"
-
 fun Called_context :: "jvm_prog \<Rightarrow> cname \<Rightarrow> instr \<Rightarrow> bool" where
 "Called_context P C\<^sub>0 (New C') = (C\<^sub>0=C')" |
 "Called_context P C\<^sub>0 (Getstatic C F D) =  ((C\<^sub>0=D) \<and> (\<exists>t. P \<turnstile> C has F,Static:t in D))" |
@@ -46,10 +41,13 @@ fun Called_context :: "jvm_prog \<Rightarrow> cname \<Rightarrow> instr \<Righta
    = (\<exists>Ts T m D. (C\<^sub>0=D) \<and> P \<turnstile> C sees M,Static:Ts \<rightarrow> T = m in D)" |
 "Called_context P _ _ = False"
 
+abbreviation Called_set :: "instr set" where
+"Called_set \<equiv> {i. \<exists>C. i = New C} \<union> {i. \<exists>C M n. i = Invokestatic C M n}
+                 \<union> {i. \<exists>C F D. i = Getstatic C F D} \<union> {i. \<exists>C F D. i = Putstatic C F D}"
+
 lemma Called_context_Called_set:
  "Called_context P D i \<Longrightarrow> i \<in> Called_set" by(cases i, auto)
 
-(* HERE: MOVE *)
 fun valid_ics :: "jvm_prog \<Rightarrow> heap \<Rightarrow> sheap \<Rightarrow> cname \<times> mname \<times> pc \<times> init_call_status \<Rightarrow> bool"
   ("_,_,_ \<turnstile>\<^sub>i _" [51,51,51,51] 50) where
 "valid_ics P h sh (C,M,pc,Calling C' Cs)
@@ -102,7 +100,6 @@ fun frame_clinit_classes :: "frame \<Rightarrow> cname list" where
 abbreviation clinit_classes :: "frame list \<Rightarrow> cname list" where
 "clinit_classes frs \<equiv> concat (map frame_clinit_classes frs)"
 
-(* HERE: MOVE? *)
 definition distinct_clinit :: "frame list \<Rightarrow> bool" where
 "distinct_clinit frs \<equiv> distinct (clinit_classes frs)"
 
@@ -110,6 +107,183 @@ definition conf_clinit :: "jvm_prog \<Rightarrow> sheap \<Rightarrow> frame list
 "conf_clinit P sh frs
    \<equiv> distinct_clinit frs \<and>
       (\<forall>C \<in> set(clinit_classes frs). is_class P C \<and> (\<exists>sfs. sh C = Some(sfs, Processing)))"
+
+(*************************)
+
+definition correct_state :: "[jvm_prog,ty\<^sub>P,jvm_state] \<Rightarrow> bool"  ("_,_ \<turnstile> _ \<surd>"  [61,0,0] 61)
+where
+  "correct_state P \<Phi> \<equiv> \<lambda>(xp,h,frs,sh).
+  case xp of
+     None \<Rightarrow> (case frs of
+             [] \<Rightarrow> True
+             | (f#fs) \<Rightarrow> P\<turnstile> h\<surd> \<and> P,h\<turnstile>\<^sub>s sh\<surd> \<and> conf_clinit P sh frs \<and>
+             (let (stk,loc,C,M,pc,ics) = f
+              in \<exists>b Ts T mxs mxl\<^sub>0 is xt \<tau>.
+                    (P \<turnstile> C sees M,b:Ts\<rightarrow>T = (mxs,mxl\<^sub>0,is,xt) in C) \<and>
+                    \<Phi> C M ! pc = Some \<tau> \<and>
+                    conf_f P h sh \<tau> is f \<and> conf_fs P h sh \<Phi> C M (size Ts) T fs))
+  | Some x \<Rightarrow> frs = []" 
+
+notation
+  correct_state  ("_,_ |- _ [ok]"  [61,0,0] 61)
+
+subsection {* Values and @{text "\<top>"} *}
+
+lemma confT_Err [iff]: "P,h \<turnstile> x :\<le>\<^sub>\<top> Err" 
+  by (simp add: confT_def)
+
+lemma confT_OK [iff]:  "P,h \<turnstile> x :\<le>\<^sub>\<top> OK T = (P,h \<turnstile> x :\<le> T)"
+  by (simp add: confT_def)
+
+lemma confT_cases:
+  "P,h \<turnstile> x :\<le>\<^sub>\<top> X = (X = Err \<or> (\<exists>T. X = OK T \<and> P,h \<turnstile> x :\<le> T))"
+  by (cases X) auto
+
+lemma confT_hext [intro?, trans]:
+  "\<lbrakk> P,h \<turnstile> x :\<le>\<^sub>\<top> T; h \<unlhd> h' \<rbrakk> \<Longrightarrow> P,h' \<turnstile> x :\<le>\<^sub>\<top> T"
+  by (cases T) (blast intro: conf_hext)+
+
+lemma confT_widen [intro?, trans]:
+  "\<lbrakk> P,h \<turnstile> x :\<le>\<^sub>\<top> T; P \<turnstile> T \<le>\<^sub>\<top> T' \<rbrakk> \<Longrightarrow> P,h \<turnstile> x :\<le>\<^sub>\<top> T'"
+  by (cases T', auto intro: conf_widen)
+
+
+subsection {* Stack and Registers *}
+
+lemmas confTs_Cons1 [iff] = list_all2_Cons1 [of "confT P h"] for P h
+
+lemma confTs_confT_sup:
+  "\<lbrakk> P,h \<turnstile> loc [:\<le>\<^sub>\<top>] LT; n < size LT; LT!n = OK T; P \<turnstile> T \<le> T' \<rbrakk> 
+  \<Longrightarrow> P,h \<turnstile> (loc!n) :\<le> T'"
+(*<*)
+  apply (frule list_all2_lengthD)
+  apply (drule list_all2_nthD, simp)
+  apply simp
+  apply (erule conf_widen, assumption+)
+  done
+(*>*)
+
+lemma confTs_hext [intro?]:
+  "P,h \<turnstile> loc [:\<le>\<^sub>\<top>] LT \<Longrightarrow> h \<unlhd> h' \<Longrightarrow> P,h' \<turnstile> loc [:\<le>\<^sub>\<top>] LT"
+  by (fast elim: list_all2_mono confT_hext)    
+
+lemma confTs_widen [intro?, trans]:
+  "P,h \<turnstile> loc [:\<le>\<^sub>\<top>] LT \<Longrightarrow> P \<turnstile> LT [\<le>\<^sub>\<top>] LT' \<Longrightarrow> P,h \<turnstile> loc [:\<le>\<^sub>\<top>] LT'"
+  by (rule list_all2_trans, rule confT_widen)
+
+lemma confTs_map [iff]:
+  "\<And>vs. (P,h \<turnstile> vs [:\<le>\<^sub>\<top>] map OK Ts) = (P,h \<turnstile> vs [:\<le>] Ts)"
+  by (induct Ts) (auto simp: list_all2_Cons2)
+
+lemma reg_widen_Err [iff]:
+  "\<And>LT. (P \<turnstile> replicate n Err [\<le>\<^sub>\<top>] LT) = (LT = replicate n Err)"
+  by (induct n) (auto simp: list_all2_Cons1)
+    
+lemma confTs_Err [iff]:
+  "P,h \<turnstile> replicate n v [:\<le>\<^sub>\<top>] replicate n Err"
+  by (induct n) auto
+
+subsection {* valid init_call_status *}
+
+lemma valid_ics_shupd:
+assumes "P,h,sh \<turnstile>\<^sub>i (C, M, pc, ics)" and "distinct (C'#ics_classes ics)"
+shows "P,h,sh(C' \<mapsto> (sfs, i')) \<turnstile>\<^sub>i (C, M, pc, ics)"
+using assms by(cases ics; clarsimp simp: fun_upd_apply) fastforce
+  
+subsection {* correct-frame *}
+
+lemma conf_f_Throwing:
+assumes "conf_f P h sh (ST, LT) is (stk, loc, C, M, pc, Called Cs)"
+  and "is_class P C'" and "h xcp = Some obj" and "sh C' = Some(sfs,Processing)"
+shows "conf_f P h sh (ST, LT) is (stk, loc, C, M, pc, Throwing (C' # Cs) xcp)"
+using assms by(auto simp: conf_f_def2)
+
+lemma conf_f_shupd:
+assumes "conf_f P h sh (ST,LT) ins f"
+ and "i = Processing
+       \<or> (distinct (C#ics_classes (ics_of f)) \<and> (curr_method f = clinit \<longrightarrow> C \<noteq> curr_class f))"
+shows "conf_f P h (sh(C \<mapsto> (sfs, i))) (ST,LT) ins f"
+using assms
+ by(cases f, cases "ics_of f"; clarsimp simp: conf_f_def2 fun_upd_apply) fastforce+
+
+lemma conf_f_shupd':
+assumes "conf_f P h sh (ST,LT) ins f"
+ and "sh C = Some(sfs,i)"
+shows "conf_f P h (sh(C \<mapsto> (sfs', i))) (ST,LT) ins f"
+using assms
+ by(cases f, cases "ics_of f"; clarsimp simp: conf_f_def2 fun_upd_apply) fastforce+
+
+subsection {* correct-frames *}
+
+lemmas [simp del] = fun_upd_apply
+
+lemma conf_fs_hext:
+  "\<And>C M n T\<^sub>r. 
+  \<lbrakk> conf_fs P h sh \<Phi> C M n T\<^sub>r frs; h \<unlhd> h' \<rbrakk> \<Longrightarrow> conf_fs P h' sh \<Phi> C M n T\<^sub>r frs"
+(*<*)
+apply (induct frs)
+ apply simp
+apply clarify
+apply (simp (no_asm_use))
+apply clarify
+apply (unfold conf_f_def)
+apply (simp (no_asm_use))
+apply clarify
+apply (fastforce elim!: confs_hext confTs_hext)
+done
+(*>*)
+
+
+lemma conf_fs_shupd:
+assumes "conf_fs P h sh \<Phi> C\<^sub>0 M n T frs"
+ and dist: "distinct (C#clinit_classes frs)"
+shows "conf_fs P h (sh(C \<mapsto> (sfs, i))) \<Phi> C\<^sub>0 M n T frs"
+using assms proof(induct frs arbitrary: C\<^sub>0 C M n T)
+  case (Cons f' frs')
+  then obtain stk' loc' C' M' pc' ics' where f': "f' = (stk',loc',C',M',pc',ics')" by(cases f')
+  with assms Cons obtain ST LT b Ts T1 mxs mxl\<^sub>0 ins xt where
+    ty: "\<Phi> C' M' ! pc' = Some (ST,LT)" and
+    meth: "P \<turnstile> C' sees M',b:Ts \<rightarrow> T1 = (mxs,mxl\<^sub>0,ins,xt) in C'" and
+    conf: "conf_f P h sh (ST, LT) ins f'" and
+    confs: "conf_fs P h sh \<Phi> C' M' (size Ts) T1 frs'" by clarsimp
+
+  from f' Cons.prems(2) have
+   "distinct (C#ics_classes (ics_of f')) \<and> (curr_method f' = clinit \<longrightarrow> C \<noteq> curr_class f')"
+     by fastforce
+  with conf_f_shupd[where C=C, OF conf] have
+    conf': "conf_f P h (sh(C \<mapsto> (sfs, i))) (ST, LT) ins f'" by simp
+
+  from Cons.prems(2) have dist': "distinct (C # clinit_classes frs')"
+    by(auto simp: distinct_length_2_or_more)
+  from Cons.hyps[OF confs dist'] have
+    confs': "conf_fs P h (sh(C \<mapsto> (sfs, i))) \<Phi> C' M' (length Ts) T1 frs'" by simp
+
+  from conf' confs' ty meth f' Cons.prems show ?case by(fastforce dest: sees_method_fun)
+qed(simp)
+
+lemma conf_fs_shupd':
+assumes "conf_fs P h sh \<Phi> C\<^sub>0 M n T frs"
+ and shC: "sh C = Some(sfs,i)"
+shows "conf_fs P h (sh(C \<mapsto> (sfs', i))) \<Phi> C\<^sub>0 M n T frs"
+using assms proof(induct frs arbitrary: C\<^sub>0 C M n T sfs i sfs')
+  case (Cons f' frs')
+  then obtain stk' loc' C' M' pc' ics' where f': "f' = (stk',loc',C',M',pc',ics')" by(cases f')
+  with assms Cons obtain ST LT b Ts T1 mxs mxl\<^sub>0 ins xt where
+    ty: "\<Phi> C' M' ! pc' = Some (ST,LT)" and
+    meth: "P \<turnstile> C' sees M',b:Ts \<rightarrow> T1 = (mxs,mxl\<^sub>0,ins,xt) in C'" and
+    conf: "conf_f P h sh (ST, LT) ins f'" and
+    confs: "conf_fs P h sh \<Phi> C' M' (size Ts) T1 frs'" and
+    shC': "sh C = Some(sfs,i)" by clarsimp
+
+  have conf': "conf_f P h (sh(C \<mapsto> (sfs', i))) (ST, LT) ins f'" by(rule conf_f_shupd'[OF conf shC'])
+
+  from Cons.hyps[OF confs shC'] have
+    confs': "conf_fs P h (sh(C \<mapsto> (sfs', i))) \<Phi> C' M' (length Ts) T1 frs'" by simp
+
+  from conf' confs' ty meth f' Cons.prems show ?case by(fastforce dest: sees_method_fun)
+qed(simp)
+
+subsection {* correctness wrt clinit use *}
 
 lemma conf_clinit_Cons:
 assumes "conf_clinit P sh (f#frs)"
@@ -167,24 +341,41 @@ assumes "conf_clinit P sh ((stk, loc, C, M, pc, ics) # frs)" and "M' \<noteq> cl
 shows "conf_clinit P sh ((stk', loc', C', M', pc', No_ics) # (stk, loc, C, M, pc, No_ics) # frs)"
  using assms conf_clinit_Cons_nclinit conf_clinit_diff' by auto
 
-(*************************)
+lemma conf_clinit_nProc_dist:
+assumes "conf_clinit P sh frs"
+  and "\<forall>sfs. sh C \<noteq> Some(sfs,Processing)"
+shows "distinct (C # clinit_classes frs)"
+using assms by(auto simp: conf_clinit_def distinct_clinit_def)
 
-definition correct_state :: "[jvm_prog,ty\<^sub>P,jvm_state] \<Rightarrow> bool"  ("_,_ \<turnstile> _ \<surd>"  [61,0,0] 61)
-where
-  "correct_state P \<Phi> \<equiv> \<lambda>(xp,h,frs,sh).
-  case xp of
-     None \<Rightarrow> (case frs of
-             [] \<Rightarrow> True
-             | (f#fs) \<Rightarrow> P\<turnstile> h\<surd> \<and> P,h\<turnstile>\<^sub>s sh\<surd> \<and> conf_clinit P sh frs \<and>
-             (let (stk,loc,C,M,pc,ics) = f
-              in \<exists>b Ts T mxs mxl\<^sub>0 is xt \<tau>.
-                    (P \<turnstile> C sees M,b:Ts\<rightarrow>T = (mxs,mxl\<^sub>0,is,xt) in C) \<and>
-                    \<Phi> C M ! pc = Some \<tau> \<and>
-                    conf_f P h sh \<tau> is f \<and> conf_fs P h sh \<Phi> C M (size Ts) T fs))
-  | Some x \<Rightarrow> frs = []" 
 
-notation
-  correct_state  ("_,_ |- _ [ok]"  [61,0,0] 61)
+lemma conf_clinit_shupd:
+assumes "conf_clinit P sh frs"
+ and dist: "distinct (C#clinit_classes frs)"
+shows "conf_clinit P (sh(C \<mapsto> (sfs, i))) frs"
+using assms by(simp add: conf_clinit_def fun_upd_apply)
+
+lemma conf_clinit_shupd':
+assumes "conf_clinit P sh frs"
+ and "sh C = Some(sfs,i)"
+shows "conf_clinit P (sh(C \<mapsto> (sfs', i))) frs"
+using assms by(fastforce simp: conf_clinit_def fun_upd_apply)
+
+lemma conf_clinit_shupd_Called:
+assumes "conf_clinit P sh ((stk,loc,C,M,pc,Calling C' Cs)#frs)"
+ and dist: "distinct (C'#clinit_classes ((stk,loc,C,M,pc,Calling C' Cs)#frs))"
+ and cls: "is_class P C'"
+shows "conf_clinit P (sh(C' \<mapsto> (sfs, Processing))) ((stk,loc,C,M,pc,Called (C'#Cs))#frs)"
+using assms by(clarsimp simp: conf_clinit_def fun_upd_apply distinct_clinit_def)
+
+lemma conf_clinit_shupd_Calling:
+assumes "conf_clinit P sh ((stk,loc,C,M,pc,Calling C' Cs)#frs)"
+ and dist: "distinct (C'#clinit_classes ((stk,loc,C,M,pc,Calling C' Cs)#frs))"
+ and cls: "is_class P C'"
+shows "conf_clinit P (sh(C' \<mapsto> (sfs, Processing)))
+         ((stk,loc,C,M,pc,Calling (fst(the(class P C'))) (C'#Cs))#frs)"
+using assms by(clarsimp simp: conf_clinit_def fun_upd_apply distinct_clinit_def)
+
+subsection {* correct state *}
 
 lemma correct_state_Cons:
 assumes cr: "P,\<Phi> |- (xp,h,f#frs,sh) [ok]"
@@ -197,118 +388,47 @@ proof -
   with cr show ?thesis by(cases frs; fastforce simp: correct_state_def)
 qed
 
-(* HERE: MOVE *) (* HERE: currently unused -- and with conf_clinit, now much more obvious *) (*
-lemma clinit_class_Proc:
- "\<lbrakk> P,\<Phi> |- (xp,h,f#frs,sh) [ok];
-    C\<^sub>0 \<in> set(clinit_classes frs) \<rbrakk>
- \<Longrightarrow> \<exists>sfs. sh C\<^sub>0 = \<lfloor>(sfs, Processing)\<rfloor>"
-proof(induct frs arbitrary: f)
-  case Nil then show ?case by(cases "curr_method f = clinit", auto simp: correct_state_def conf_f_def2)
-next
-  case (Cons f' frs')
-  with correct_state_Cons[OF Cons.prems(1)] have
-   cr': "P,\<Phi> |- (xp,h,f'#frs',sh) [ok]" by simp
+(* HERE: unused *)
+lemma correct_state_shupd:
+assumes cs: "P,\<Phi> |- (xp,h,frs,sh) [ok]" and shC: "sh C = Some(sfs,i)"
+ and dist: "distinct (C#clinit_classes frs)"
+shows "P,\<Phi> |- (xp,h,frs,sh(C \<mapsto> (sfs, i'))) [ok]"
+using assms
+proof(cases xp)
+  case None with assms show ?thesis
+  proof(cases frs)
+    case (Cons f' frs')
+    let ?sh = "sh(C \<mapsto> (sfs, i'))"
 
-  show ?case
-  proof(cases "C\<^sub>0 \<in> set(frame_clinit_classes f')")
-    case False with cr' Cons show ?thesis by simp
-  next
-    case True with Cons.prems(1) show ?thesis
-      by(auto simp: correct_state_def conf_f_def2 conf_clinit_def)
-  qed
-qed *)
+    obtain stk' loc' C' M' pc' ics' where f': "f' = (stk',loc',C',M',pc',ics')" by(cases f')
+    with cs Cons None obtain b Ts T mxs mxl\<^sub>0 ins xt ST LT where
+         meth: "P \<turnstile> C' sees M',b:Ts\<rightarrow>T = (mxs,mxl\<^sub>0,ins,xt) in C'"
+     and ty: "\<Phi> C' M' ! pc' = Some (ST,LT)" and conf: "conf_f P h sh (ST,LT) ins f'"
+     and confs: "conf_fs P h sh \<Phi> C' M' (size Ts) T frs'"
+     and confc: "conf_clinit P sh frs"
+     and h_ok: "P\<turnstile> h\<surd>" and sh_ok: "P,h \<turnstile>\<^sub>s sh \<surd>"
+    by(auto simp: correct_state_def)
 
-(* HERE: MOVE *) (* HERE: not used
-(* if C is not in a current clinit state, then C has no current clinit frame *)
-lemma nclinit_current:
-assumes cr: "P,\<Phi> |- (xp,h,(stk,loc,C,M,pc,ics)#frs,sh) [ok]"
-    and ncc: "\<not>clinit_current sh C\<^sub>0 clinit"
-shows "distinct (C\<^sub>0#clinit_classes ((stk,loc,C,M,pc,ics)#frs))"
-proof -
-  from cr have dist: "distinct_clinit ((stk,loc,C,M,pc,ics)#frs)"
-    by(cases "M=clinit"; clarsimp simp: correct_state_def)
-  { assume "C\<^sub>0 \<in> set(clinit_classes ((stk,loc,C,M,pc,ics)#frs))"
-    with clinit_class_Proc[OF cr] ncc have "False" by auto
-  }
-  then have "C\<^sub>0 \<notin> set(clinit_classes ((stk,loc,C,M,pc,ics)#frs))" by fast
-  with dist show ?thesis by simp
-qed *)
+    from Cons dist have dist': "distinct (C#clinit_classes frs')"
+     by(auto simp: distinct_length_2_or_more)
 
-subsection {* Values and @{text "\<top>"} *}
+    from shconf_upd_obj[OF sh_ok shconfD[OF sh_ok shC]] have sh_ok': "P,h \<turnstile>\<^sub>s ?sh \<surd>"
+      by simp
 
-lemma confT_Err [iff]: "P,h \<turnstile> x :\<le>\<^sub>\<top> Err" 
-  by (simp add: confT_def)
+    from conf f' valid_ics_shupd Cons dist have conf': "conf_f P h ?sh (ST,LT) ins f'"
+     by(auto simp: conf_f_def2 fun_upd_apply)
+    have confs': "conf_fs P h ?sh \<Phi> C' M' (size Ts) T frs'" by(rule conf_fs_shupd[OF confs dist'])
 
-lemma confT_OK [iff]:  "P,h \<turnstile> x :\<le>\<^sub>\<top> OK T = (P,h \<turnstile> x :\<le> T)"
-  by (simp add: confT_def)
+    have confc': "conf_clinit P ?sh frs" by(rule conf_clinit_shupd[OF confc dist])
 
-lemma confT_cases:
-  "P,h \<turnstile> x :\<le>\<^sub>\<top> X = (X = Err \<or> (\<exists>T. X = OK T \<and> P,h \<turnstile> x :\<le> T))"
-  by (cases X) auto
+    with h_ok sh_ok' meth ty conf' confs' f' Cons None show ?thesis
+     by(fastforce simp: correct_state_def)
+  qed(simp add: correct_state_def)
+qed(simp add: correct_state_def)
 
-lemma confT_hext [intro?, trans]:
-  "\<lbrakk> P,h \<turnstile> x :\<le>\<^sub>\<top> T; h \<unlhd> h' \<rbrakk> \<Longrightarrow> P,h' \<turnstile> x :\<le>\<^sub>\<top> T"
-  by (cases T) (blast intro: conf_hext)+
-
-lemma confT_widen [intro?, trans]:
-  "\<lbrakk> P,h \<turnstile> x :\<le>\<^sub>\<top> T; P \<turnstile> T \<le>\<^sub>\<top> T' \<rbrakk> \<Longrightarrow> P,h \<turnstile> x :\<le>\<^sub>\<top> T'"
-  by (cases T', auto intro: conf_widen)
-
-
-subsection {* Stack and Registers *}
-
-lemmas confTs_Cons1 [iff] = list_all2_Cons1 [of "confT P h"] for P h
-
-lemma confTs_confT_sup:
-  "\<lbrakk> P,h \<turnstile> loc [:\<le>\<^sub>\<top>] LT; n < size LT; LT!n = OK T; P \<turnstile> T \<le> T' \<rbrakk> 
-  \<Longrightarrow> P,h \<turnstile> (loc!n) :\<le> T'"
-(*<*)
-  apply (frule list_all2_lengthD)
-  apply (drule list_all2_nthD, simp)
-  apply simp
-  apply (erule conf_widen, assumption+)
-  done
-(*>*)
-
-lemma confTs_hext [intro?]:
-  "P,h \<turnstile> loc [:\<le>\<^sub>\<top>] LT \<Longrightarrow> h \<unlhd> h' \<Longrightarrow> P,h' \<turnstile> loc [:\<le>\<^sub>\<top>] LT"
-  by (fast elim: list_all2_mono confT_hext)    
-
-lemma confTs_widen [intro?, trans]:
-  "P,h \<turnstile> loc [:\<le>\<^sub>\<top>] LT \<Longrightarrow> P \<turnstile> LT [\<le>\<^sub>\<top>] LT' \<Longrightarrow> P,h \<turnstile> loc [:\<le>\<^sub>\<top>] LT'"
-  by (rule list_all2_trans, rule confT_widen)
-
-lemma confTs_map [iff]:
-  "\<And>vs. (P,h \<turnstile> vs [:\<le>\<^sub>\<top>] map OK Ts) = (P,h \<turnstile> vs [:\<le>] Ts)"
-  by (induct Ts) (auto simp add: list_all2_Cons2)
-
-lemma reg_widen_Err [iff]:
-  "\<And>LT. (P \<turnstile> replicate n Err [\<le>\<^sub>\<top>] LT) = (LT = replicate n Err)"
-  by (induct n) (auto simp add: list_all2_Cons1)
-    
-lemma confTs_Err [iff]:
-  "P,h \<turnstile> replicate n v [:\<le>\<^sub>\<top>] replicate n Err"
-  by (induct n) auto
-
-  
-subsection {* correct-frames *}
-
-lemmas [simp del] = fun_upd_apply
-
-lemma conf_fs_hext:
-  "\<And>C M n T\<^sub>r. 
-  \<lbrakk> conf_fs P h sh \<Phi> C M n T\<^sub>r frs; h \<unlhd> h' \<rbrakk> \<Longrightarrow> conf_fs P h' sh \<Phi> C M n T\<^sub>r frs"
-(*<*)
-apply (induct frs)
- apply simp
-apply clarify
-apply (simp (no_asm_use))
-apply clarify
-apply (unfold conf_f_def)
-apply (simp (no_asm_use))
-apply clarify
-apply (fastforce elim!: confs_hext confTs_hext)
-done
-(*>*)
+lemma correct_state_Throwing_ex:
+assumes correct: "P,\<Phi> \<turnstile> (xp,h,(stk,loc,C,M,pc,ics)#frs,sh)\<surd>"
+shows "\<And>Cs a. ics = Throwing Cs a \<Longrightarrow> \<exists>obj. h a = Some obj"
+using correct by(clarsimp simp: correct_state_def conf_f_def)
 
 end
