JVM/JVMExceptions.thy
@@ -3,7 +3,7 @@
     Copyright   2001 Technische Universitaet Muenchen
 *)
 (*
-  Expanded by Susannah Mansky
+  Expanded to include dynamic class initialization by Susannah Mansky
   2016-17, UIUC
 *)
 
@@ -39,24 +39,42 @@ where
          case match_ex_table P (cname_of h a) pc (ex_table_of P C M) of
            None \<Rightarrow> 
               (case M = clinit of
-                   True \<Rightarrow> (case frs of (stk',loc',C',M',pc',ics')#frs'
-                                          \<Rightarrow> (case ics' of Called Cs \<Rightarrow> (None, h, (stk',loc',C',M',pc',Throwing (C#Cs) a)#frs', sh)
-                                                         | _ \<Rightarrow> (None, h, (stk',loc',C',M',pc',ics')#frs', sh) \<comment> \<open>this won't happen in wf code\<close>
-                                             )
-                                      | [] \<Rightarrow> (Some a, h, [], sh)
-                           )
-                 | _ \<Rightarrow> find_handler P a h frs sh
+                 True \<Rightarrow> (case frs of (stk',loc',C',M',pc',ics')#frs'
+                                  \<Rightarrow> (case ics' of Called Cs \<Rightarrow> (None, h, (stk',loc',C',M',pc',Throwing (C#Cs) a)#frs', sh)
+                                                 | _ \<Rightarrow> (None, h, (stk',loc',C',M',pc',ics')#frs', sh) \<comment> \<open>this won't happen in wf code\<close>
+                                     )
+                              | [] \<Rightarrow> (Some a, h, [], sh)
+                    )
+               | _ \<Rightarrow> find_handler P a h frs sh
               )
          | Some pc_d \<Rightarrow> (None, h, (Addr a # drop (size stk - snd pc_d) stk, loc, C, M, fst pc_d, No_ics)#frs, sh))"
 
 lemma find_handler_cases:
  "find_handler P a h frs sh = js
-   \<Longrightarrow> (\<exists>frs'. frs' \<noteq> [] \<and> js = (None, h, frs', sh)) \<or> (\<exists>x. js = (Some x, h, [], sh))"
-apply (cut_tac P = "\<lambda>P a h frs sh. \<forall>js. find_handler P a h frs sh = js \<longrightarrow>
-  (\<exists>frs'. frs' \<noteq> [] \<and> js = (None, h, frs', sh)) \<or> (\<exists>x. js = (Some x, h, [], sh))"
-  and ?a0.0 = P and ?a1.0 = a and ?a2.0 = h and ?a3.0 = frs and ?a4.0 = sh
- in find_handler.induct)
-by(auto split: bool.splits list.splits init_call_status.splits)
+  \<Longrightarrow> (\<exists>frs'. frs' \<noteq> [] \<and> js = (None, h, frs', sh)) \<or> (js = (Some a, h, [], sh))"
+proof(induct P a h frs sh rule: find_handler.induct)
+  case 1 then show ?case by clarsimp
+next
+  case (2 P a h fr frs sh) then show ?case
+    by(cases fr, auto split: bool.splits list.splits init_call_status.splits)
+qed
+
+lemma find_handler_heap[simp]:
+"find_handler P a h frs sh = (xp',h',frs',sh') \<Longrightarrow> h' = h"
+ by(auto dest: find_handler_cases)
+
+lemma find_handler_sheap[simp]:
+"find_handler P a h frs sh = (xp',h',frs',sh') \<Longrightarrow> sh' = sh"
+ by(auto dest: find_handler_cases)
+
+lemma find_handler_frames[simp]:
+"find_handler P a h frs sh = (xp',h',frs',sh') \<Longrightarrow> length frs' \<le> length frs"
+proof(induct frs)
+  case Nil then show ?case by simp
+next
+  case (Cons a frs) then show ?case
+    by(auto simp: split_beta split: bool.splits list.splits init_call_status.splits)
+qed
 
 lemma find_handler_None:
  "find_handler P a h frs sh = (None, h, frs', sh') \<Longrightarrow> frs' \<noteq> []"
@@ -68,23 +86,14 @@ lemma find_handler_Some:
 
 lemma find_handler_Some_same_error_same_heap[simp]:
  "find_handler P a h frs sh = (Some x, h', frs', sh') \<Longrightarrow> x = a \<and> h = h' \<and> sh = sh'"
-apply (cut_tac P = "\<lambda>P a h frs sh. find_handler P a h frs sh = (Some x, h', frs', sh') \<longrightarrow>
-   x = a \<and> h = h' \<and> sh = sh'"
-  and ?a0.0 = P and ?a1.0 = a and ?a2.0 = h and ?a3.0 = frs and ?a4.0 = sh
- in find_handler.induct)
-by(auto split: bool.splits list.splits init_call_status.splits)
+ by(auto dest: find_handler_cases)
 
-lemma find_handler_frames[simp]:
-"find_handler P a h frs sh = (xp',h',frs',sh') \<Longrightarrow> length frs' \<le> length frs"
-proof(induct frs)
-  case Nil then show ?case by simp
-next
-  case (Cons a frs)
-  then show ?case
-    by(auto simp: split_beta split: bool.splits list.splits init_call_status.splits)
-qed
+lemma find_handler_prealloc_pres:
+assumes "preallocated h"
+and fh: "find_handler P a h frs sh = (xp',h',frs',sh')"
+shows "preallocated h'"
+using assms find_handler_heap[OF fh] by simp
 
-(* HERE: MOVE *)
 lemma find_handler_frs_tl_neq:
  "ics_of f \<noteq> No_ics
   \<Longrightarrow> (xp, h, f#frs, sh) \<noteq> find_handler P xa h' (f' # frs) sh'"
@@ -101,33 +110,19 @@ next
   proof(cases "find_handler P xa h' (f' # a # frs) sh' = find_handler P xa h' (a # frs) sh'")
     case True then show ?thesis using neq fh by simp
   next
-    case False
-    then show ?thesis using Cons.prems
-      by(auto simp: split_beta split: bool.splits init_call_status.splits list.splits)
+    case False then show ?thesis using Cons.prems
+      by(fastforce simp: split_beta split: bool.splits init_call_status.splits list.splits)
   qed
 qed
 
-lemma find_handler_heap[simp]:
-"find_handler P a h frs sh = (xp',h',frs',sh') \<Longrightarrow> h' = h"
- by(auto dest: find_handler_cases)
-
-lemma find_handler_prealloc_pres:
-assumes "preallocated h"
-and fh: "find_handler P a h frs sh = (xp',h',frs',sh')"
-shows "preallocated h'"
-using assms find_handler_heap[OF fh] by simp
-
-lemma find_handler_sheap[simp]:
-"find_handler P a h frs sh = (xp',h',frs',sh') \<Longrightarrow> sh' = sh"
- by(auto dest: find_handler_cases)
-
+(* HERE: true, but unused
 lemma find_handler_sheap_no_effect:
 assumes "find_handler P a h frs sh = (xp',h',frs',sh')"
 shows "find_handler P a h frs sh1 = (xp',h',frs',sh1)"
 using assms proof(induct frs)
-  case (Cons f' frs')
-  then obtain stk' loc' C' M' pc' ics' where "f'=(stk',loc',C',M',pc',ics')" by(cases f')
-  with Cons show ?case by(auto split: bool.splits list.splits init_call_status.splits)
+  case (Cons f' frs') then show ?case
+    by(cases f', auto split: bool.splits list.splits init_call_status.splits)
 qed(simp)
+*)
 
 end
